PsNat.v
@@ -6,108 +6,108 @@ Require Import Omega.
 Require Import Listutils.
 Require Import PsCore.
 
-Definition termincr : term := termseq
-  [ termdup ; termquote ; termswap ; termquote ; termcons ;
-    termswap ; termquote ; termcons ; termexec ;
-    termsnoc ; termswap ].
+Definition instincr : inst := instseq
+  [ instdup ; instquote ; instswap ; instquote ; instcons ;
+    instswap ; instquote ; instcons ; instexec ;
+    instsnoc ; instswap ].
 
-Lemma eval_termincr : forall (t1 t2 : term) (vs ps : stack),
-  (t1 :: t2 :: vs, termincr :: ps) |=>* (t1 :: termpair t2 t1 :: vs, ps).
+Lemma eval_instincr : forall (i1 i2 : inst) (vs ps : stack),
+  (i1 :: i2 :: vs, instincr :: ps) |=>* (i1 :: instpair i2 i1 :: vs, ps).
   intros ; evalauto.
 Qed.
 
-Lemma eval_termincr_replicate : forall (n : nat) (t1 t2 : term) (vs ps : stack),
-  (t1 :: t2 :: vs, replicate n termincr ++ ps) |=>*
-    (t1 :: termseq' (replicate n t1) t2 :: vs, ps).
+Lemma eval_instincr_replicate : forall (n : nat) (i1 i2 : inst) (vs ps : stack),
+  (i1 :: i2 :: vs, replicate n instincr ++ ps) |=>*
+    (i1 :: instseq' (replicate n i1) i2 :: vs, ps).
   induction n ; intros ; evalauto.
   evalpartial IHn ; evalauto.
 Qed.
 
-Definition termnatq (n : nat) : term := termseq (replicate n termincr).
+Definition instnatq (n : nat) : inst := instseq (replicate n instincr).
 
-Lemma eval_termnatq : forall (n : nat) (t1 t2 : term) (vs ps : stack),
-  (t1 :: t2 :: vs, termnatq n :: ps) |=>*
-    (t1 :: termseq' (replicate n t1) t2 :: vs, ps).
+Lemma eval_instnatq : forall (n : nat) (i1 i2 : inst) (vs ps : stack),
+  (i1 :: i2 :: vs, instnatq n :: ps) |=>*
+    (i1 :: instseq' (replicate n i1) i2 :: vs, ps).
   intros.
-  evalpartial eval_termseq.
-  evalpartial eval_termincr_replicate.
+  evalpartial evalseq.
+  evalpartial eval_instincr_replicate.
   evalauto.
 Qed.
 
-Definition termnat_spec (n : nat) (t1 : term) : Prop :=
-  forall (t2 : term) (vs ps : stack),
-    (t2 :: vs, t1 :: ps) |=>* (vs, replicate n t2 ++ ps).
+Definition instnat_spec (n : nat) (i1 : inst) : Prop :=
+  forall (i2 : inst) (vs ps : stack),
+    (i2 :: vs, i1 :: ps) |=>* (vs, replicate n i2 ++ ps).
 
-Definition termnat (n : nat) : term := termseq
-  [ termpush ; termnop ; termswap ; termnatq n ; termpop ; termexec ].
+Definition instnat (n : nat) : inst := instseq
+  [ instpush ; instnop ; instswap ; instnatq n ; instpop ; instexec ].
 
-Lemma eval_termnat : forall (n : nat), termnat_spec n (termnat n).
+Lemma eval_instnat : forall (n : nat), instnat_spec n (instnat n).
   repeat intro.
-  evalpartial eval_termseq ; evalauto.
-  evalpartial eval_termnatq ; evalauto.
-  apply eval_termseq.
+  evalpartial evalseq ; evalauto.
+  evalpartial eval_instnatq ; evalauto.
+  apply evalseq.
 Qed.
 
-Definition termnat_quote : term := termseq
-  [ termpush ; termnop ; termquote ;
-    termpush ; termincr ; termquote ; termcons ;
-    termswap ; termquote ; termcons ; termexec ;
-    termpush ; termincr ; termswap ; termexec ; termpop ].
+Definition instnat_quote : inst := instseq
+  [ instpush ; instnop ; instquote ;
+    instpush ; instincr ; instquote ; instcons ;
+    instswap ; instquote ; instcons ; instexec ;
+    instpush ; instincr ; instswap ; instexec ; instpop ].
 
-Lemma eval_termnat_quote :
-  forall (n : nat) (t : term) (vs ps : stack), termnat_spec n t ->
-    (t :: vs, termnat_quote :: ps) |=>* (termnatq n :: vs, ps).
+Lemma eval_instnat_quote :
+  forall (n : nat) (i : inst) (vs ps : stack), instnat_spec n i ->
+    (i :: vs, instnat_quote :: ps) |=>* (instnatq n :: vs, ps).
   repeat intro.
-  evalauto ; evalpartial H ; evalpartial eval_termincr_replicate ; evalauto.
+  evalauto ; evalpartial H ; evalpartial eval_instincr_replicate ; evalauto.
 Qed.
 
-Definition termnat_unquote : term := termseq
-  [ termpush ; termnop ;
-    termpush ; termpush ; termcons ;
-    termpush ; termnop ; termcons ;
-    termpush ; termswap ; termcons ;
-    termsnoc ;
-    termpush ; termpop ; termcons ;
-    termpush ; termexec ; termcons ].
+Definition instnat_unquote : inst := instseq
+  [ instpush ; instnop ;
+    instpush ; instpush ; instcons ;
+    instpush ; instnop ; instcons ;
+    instpush ; instswap ; instcons ;
+    instsnoc ;
+    instpush ; instpop ; instcons ;
+    instpush ; instexec ; instcons ].
 
-Definition eval_termnat_unquote : forall (n : nat) (vs ps : stack),
-  (termnatq n :: vs, termnat_unquote :: ps) |=>* (termnat n :: vs, ps).
+Definition eval_instnat_unquote : forall (n : nat) (vs ps : stack),
+  (instnatq n :: vs, instnat_unquote :: ps) |=>* (instnat n :: vs, ps).
   repeat intro ; evalauto.
 Qed.
 
-Lemma termnatq_eqmap : forall (n m : nat), termnatq n = termnatq m -> n = m.
+Lemma instnatq_eqmap : forall (n m : nat), instnatq n = instnatq m -> n = m.
   intro.
   induction n ; intros ; destruct m.
   auto.
-  unfold termnatq, termseq, replicate at 1, termseq' at 1, fold_left in H.
-  rewrite (termseq_replicate (S m) termincr termnop) in H.
+  unfold instnatq, instseq, replicate at 1, instseq' at 1, fold_left in H.
+  rewrite (instseq_replicate (S m) instincr instnop) in H.
   inversion H.
-  unfold termnatq, termseq, replicate at 2, termseq' at 2, fold_left in H.
-  rewrite (termseq_replicate (S n) termincr termnop) in H.
+  unfold instnatq, instseq, replicate at 2, instseq' at 2, fold_left in H.
+  rewrite (instseq_replicate (S n) instincr instnop) in H.
   inversion H.
   f_equal.
   apply IHn.
-  unfold termnatq, termseq in *.
-  repeat erewrite termseq_replicate in *.
+  unfold instnatq, instseq in *.
+  repeat erewrite instseq_replicate in *.
   inversion H.
   auto.
 Qed.
 
-Lemma termnat_eqmap : forall (n m : nat) (t : term),
-  termnat_spec n t -> termnat_spec m t -> n = m.
+Lemma instnat_eqmap : forall (n m : nat) (i : inst),
+  instnat_spec n i -> instnat_spec m i -> n = m.
   intros.
   assert
-    (([], replicate n termpop) |=>*' ([], replicate m termpop) \/
-     ([], replicate m termpop) |=>*' ([], replicate n termpop)).
+    (([], replicate n instpop) |=>*' ([], replicate m instpop) \/
+     ([], replicate m instpop) |=>*' ([], replicate n instpop)).
     repeat erewrite <- evalrtc_is_evalrtc'.
-    apply (@evalrtc_confluence ([ termpop ], [ t ])).
+    apply (@evalrtc_confluence ([ instpop ], [ i ])).
     evalpartial H.
     erewrite app_nil_r.
     evalauto.
     evalpartial H0.
     erewrite app_nil_r.
     evalauto.
-  assert (replicate n termpop = replicate m termpop).
+  assert (replicate n instpop = replicate m instpop).
     destruct H1 ; destruct n ; destruct m ; inversion H1 ;
       (auto || inversion H2 || simpl ; f_equal ; auto).
   clear H H0 H1.
@@ -115,153 +115,153 @@ Lemma termnat_eqmap : forall (n m : nat) (t : term),
     (auto || congruence || f_equal ; apply IHn ; congruence).
 Qed.
 
-Definition termnatq_succ : term :=
-  termseq [ termpush ; termincr ; termcons ].
+Definition instnatq_succ : inst :=
+  instseq [ instpush ; instincr ; instcons ].
 
-Lemma eval_termnatq_succ : forall (n : nat) (vs ps : stack),
-  (termnatq n :: vs, termnatq_succ :: ps) |=>* (termnatq (S n) :: vs, ps).
+Lemma eval_instnatq_succ : forall (n : nat) (vs ps : stack),
+  (instnatq n :: vs, instnatq_succ :: ps) |=>* (instnatq (S n) :: vs, ps).
   intros.
   evalauto.
   rtcequal.
-  unfold termnat, termnatq, termseq.
-  erewrite termseq_replicate.
+  unfold instnat, instnatq, instseq.
+  erewrite instseq_replicate.
   simpl ; unfold flip ; f_equal.
-  apply eq_sym, termseq_replicate.
+  apply eq_sym, instseq_replicate.
 Qed.
 
-Lemma eval_termnatq_succ_replicate : forall (n m : nat) (vs ps : stack),
-  (termnatq n :: vs, replicate m termnatq_succ ++ ps) |=>*
-    (termnatq (m + n) :: vs, ps).
+Lemma eval_instnatq_succ_replicate : forall (n m : nat) (vs ps : stack),
+  (instnatq n :: vs, replicate m instnatq_succ ++ ps) |=>*
+    (instnatq (m + n) :: vs, ps).
   intros ; revert n.
   induction m ; intros.
   evalauto.
   simpl.
-  evalpartial eval_termnatq_succ.
+  evalpartial eval_instnatq_succ.
   evalpartial IHm.
   rtcequal ; omega.
 Qed.
 
-Definition termnat_succ : term :=
-  termseq [ termnat_quote ; termnatq_succ ; termnat_unquote ].
+Definition instnat_succ : inst :=
+  instseq [ instnat_quote ; instnatq_succ ; instnat_unquote ].
 
-Lemma eval_termnat_succ :
-  forall (n : nat) (t : term) (vs ps : stack), termnat_spec n t ->
-    (t :: vs, termnat_succ :: ps) |=>* (termnat (S n) :: vs, ps).
+Lemma eval_instnat_succ :
+  forall (n : nat) (i : inst) (vs ps : stack), instnat_spec n i ->
+    (i :: vs, instnat_succ :: ps) |=>* (instnat (S n) :: vs, ps).
   intros.
-  evalpartial eval_termseq.
-  evalpartial' eval_termnat_quote.
+  evalpartial evalseq.
+  evalpartial' eval_instnat_quote.
   apply H.
-  evalpartial eval_termnatq_succ.
+  evalpartial eval_instnatq_succ.
   evalauto.
 Qed.
 
-Lemma termnat_succ_proof :
-  forall (n : nat) (t1 : term) (vs ps : stack), termnat_spec n t1 ->
-    exists t2 : term, termnat_spec (S n) t2 /\
-      (t1 :: vs, termnat_succ :: ps) |=>* (t2 :: vs, ps).
+Lemma instnat_succ_proof :
+  forall (n : nat) (i1 : inst) (vs ps : stack), instnat_spec n i1 ->
+    exists i2 : inst, instnat_spec (S n) i2 /\
+      (i1 :: vs, instnat_succ :: ps) |=>* (i2 :: vs, ps).
   intros.
-  exists (termnat (S n)).
+  exists (instnat (S n)).
   split.
-  apply eval_termnat.
-  apply eval_termnat_succ ; auto.
+  apply eval_instnat.
+  apply eval_instnat_succ ; auto.
 Qed.
 
-Definition termnatq_add : term :=
-  termseq [ termpush ; termincr ; termswap ; termexec ; termpop ].
+Definition instnatq_add : inst :=
+  instseq [ instpush ; instincr ; instswap ; instexec ; instpop ].
 
-Lemma eval_termnatq_add : forall (n m : nat) (vs ps : stack),
-  (termnatq m :: termnatq n :: vs, termnatq_add :: ps) |=>*
-    (termnatq (n + m) :: vs, ps).
+Lemma eval_instnatq_add : forall (n m : nat) (vs ps : stack),
+  (instnatq m :: instnatq n :: vs, instnatq_add :: ps) |=>*
+    (instnatq (n + m) :: vs, ps).
   intros.
   evalauto.
-  evalpartial eval_termnatq.
+  evalpartial eval_instnatq.
   evalauto.
-  unfold termnatq.
-  erewrite <- app_termseq, replicate_app.
+  unfold instnatq.
+  erewrite <- app_instseq, replicate_app.
   evalauto.
 Qed.
 
-Definition termnat_add : term := termseq
-  [ termnat_quote ; termswap ;
-    termpush ; termnatq_succ ; termswap ; termexec ; termnat_unquote ].
+Definition instnat_add : inst := instseq
+  [ instnat_quote ; instswap ;
+    instpush ; instnatq_succ ; instswap ; instexec ; instnat_unquote ].
 
-Lemma eval_termnat_add : forall (n m : nat) (t1 t2 : term) (vs ps : stack),
-  termnat_spec n t1 -> termnat_spec m t2 ->
-    (t2 :: t1 :: vs, termnat_add :: ps) |=>* (termnat (n + m) :: vs, ps).
+Lemma eval_instnat_add : forall (n m : nat) (i1 i2 : inst) (vs ps : stack),
+  instnat_spec n i1 -> instnat_spec m i2 ->
+    (i2 :: i1 :: vs, instnat_add :: ps) |=>* (instnat (n + m) :: vs, ps).
   intros.
-  evalpartial eval_termseq.
-  evalpartial' eval_termnat_quote.
+  evalpartial evalseq.
+  evalpartial' eval_instnat_quote.
   apply H0.
   evalauto.
   evalpartial H.
-  evalpartial eval_termnatq_succ_replicate.
-  apply eval_termnat_unquote.
+  evalpartial eval_instnatq_succ_replicate.
+  apply eval_instnat_unquote.
 Qed.
 
-Lemma termnat_add_proof : forall (n m : nat) (t1 t2 : term) (vs ps : stack),
-  termnat_spec n t1 -> termnat_spec m t2 ->
-    exists t3 : term, termnat_spec (n + m) t3 /\
-      (t2 :: t1 :: vs, termnat_add :: ps) |=>* (t3 :: vs, ps).
+Lemma instnat_add_proof : forall (n m : nat) (i1 i2 : inst) (vs ps : stack),
+  instnat_spec n i1 -> instnat_spec m i2 ->
+    exists i3 : inst, instnat_spec (n + m) i3 /\
+      (i2 :: i1 :: vs, instnat_add :: ps) |=>* (i3 :: vs, ps).
   intros.
   eexists.
   split.
-  apply eval_termnat.
-  apply eval_termnat_add ; auto.
+  apply eval_instnat.
+  apply eval_instnat_add ; auto.
 Qed.
 
-Definition termnatq_mult : term := termseq
-  [ termpush ; termnop ; termpush ; termpush ; termcons ; termsnoc ;
-    termpush ; termnatq_add ; termcons ; termquote ;
-    termpush ; termnatq 0 ; termquote ; termsnoc ;
-    termswap ; termnat_unquote ; termcons ; termexec ].
+Definition instnatq_mult : inst := instseq
+  [ instpush ; instnop ; instpush ; instpush ; instcons ; instsnoc ;
+    instpush ; instnatq_add ; instcons ; instquote ;
+    instpush ; instnatq 0 ; instquote ; instsnoc ;
+    instswap ; instnat_unquote ; instcons ; instexec ].
 
-Lemma eval_termnatq_mult : forall (n m : nat) (vs ps : stack),
-  (termnatq m :: termnatq n :: vs, termnatq_mult :: ps) |=>*
-    (termnatq (n * m) :: vs, ps).
+Lemma eval_instnatq_mult : forall (n m : nat) (vs ps : stack),
+  (instnatq m :: instnatq n :: vs, instnatq_mult :: ps) |=>*
+    (instnatq (n * m) :: vs, ps).
   intros.
   do 126 evalstep.
-  evalpartial eval_termnat.
-  assert (forall (a : nat), (termnatq a :: vs,
-    replicate n (termseq [ termpush ; termnatq m ; termnatq_add ]) ++ ps)
-      |=>* (termnatq (a + n * m) :: vs, ps)).
+  evalpartial eval_instnat.
+  assert (forall (a : nat), (instnatq a :: vs,
+    replicate n (instseq [ instpush ; instnatq m ; instnatq_add ]) ++ ps)
+      |=>* (instnatq (a + n * m) :: vs, ps)).
     induction n ; intros.
     replace (a + 0 * m) with a by omega.
     evalauto.
     simpl.
-    evalpartial eval_termseq.
+    evalpartial evalseq.
     evalstep.
-    evalpartial eval_termnatq_add.
+    evalpartial eval_instnatq_add.
     replace (a + (m + n * m)) with ((a + m) + n * m) by omega.
     apply IHn.
   evalpartial (H 0) ; evalauto.
 Qed.
 
-Definition termnat_mult : term := termseq
-  [ termnat_quote ; termswap ; termnat_quote ; termswap ;
-    termnatq_mult ; termnat_unquote ].
+Definition instnat_mult : inst := instseq
+  [ instnat_quote ; instswap ; instnat_quote ; instswap ;
+    instnatq_mult ; instnat_unquote ].
 
-Lemma eval_termnat_mult : forall (n m : nat) (t1 t2 : term) (vs ps : stack),
-  termnat_spec n t1 -> termnat_spec m t2 ->
-    (t2 :: t1 :: vs, termnat_mult :: ps) |=>* (termnat (n * m) :: vs, ps).
+Lemma eval_instnat_mult : forall (n m : nat) (i1 i2 : inst) (vs ps : stack),
+  instnat_spec n i1 -> instnat_spec m i2 ->
+    (i2 :: i1 :: vs, instnat_mult :: ps) |=>* (instnat (n * m) :: vs, ps).
   intros.
-  evalpartial eval_termseq.
-  evalpartial' eval_termnat_quote.
+  evalpartial evalseq.
+  evalpartial' eval_instnat_quote.
   apply H0.
   evalstep.
-  evalpartial' eval_termnat_quote.
+  evalpartial' eval_instnat_quote.
   apply H.
   evalstep.
-  evalpartial eval_termnatq_mult.
-  apply eval_termnat_unquote.
+  evalpartial eval_instnatq_mult.
+  apply eval_instnat_unquote.
 Qed.
 
-Lemma termnat_mult_proof : forall (n m : nat) (t1 t2 : term) (vs ps : stack),
-  termnat_spec n t1 -> termnat_spec m t2 ->
-    exists t3 : term, termnat_spec (n * m) t3 /\
-      (t2 :: t1 :: vs, termnat_mult :: ps) |=>* (t3 :: vs, ps).
+Lemma instnat_mult_proof : forall (n m : nat) (i1 i2 : inst) (vs ps : stack),
+  instnat_spec n i1 -> instnat_spec m i2 ->
+    exists i3 : inst, instnat_spec (n * m) i3 /\
+      (i2 :: i1 :: vs, instnat_mult :: ps) |=>* (i3 :: vs, ps).
   intros.
   eexists.
   split.
-  apply eval_termnat.
-  apply eval_termnat_mult ; auto.
+  apply eval_instnat.
+  apply eval_instnat_mult ; auto.
 Qed.
